세 가지 성질을 증명하면 된다.
## $\mu_Y(\emptyset) = 0$
$$\mu_Y(\emptyset) = \mu_X(f^{-1}(\emptyset)) = \mu_X(\emptyset) = 0$$
## $\mu_Y(E) \ge 0$
$$\mu_Y(E) = \mu_X(f^{-1}(E)) \ge 0$$
## $\mu_Y{\left(\biguplus_{i=1}^\infin A_i\right)} = \sum_{i=1}^\infin\mu_Y(A_i)$
$$\mu_Y{\left(\biguplus_{i=1}^\infin A_i\right)}
\\=\mu_X\left(f^{-1}\left(\biguplus_{i=1}^\infin A_i\right)\right)
\\= \mu_X \left(\biguplus_{i=1}^\infin f^{-1} (A_i)\right)
\\= \sum_{i=1}^\infin\mu_X(f^{-1}(A_i))
\\=\sum_{i=1}^\infin\mu_Y(A_i)
$$