$v = 0$인 경우 자명하다.

$v \neq 0$인 경우
$$
z := u - {\langle u,v \rangle \over \langle v, v\rangle}v
$$
에 대해
$$
\langle v, z\rangle= \langle v, u - {\langle u,v \rangle \over \langle v, v\rangle}v\rangle = \langle u, v\rangle - {\langle u,v \rangle \over \langle v, v\rangle} \langle v,v\rangle = 0
$$
이다.

$v$와 $z$가 직교하므로 $u = z + {\langle u,v \rangle \over \langle v, v\rangle}v$에 대해 Pythagorean Theorem을 사용하면
$$
\langle u,u\rangle =\langle z ,z\rangle + |{\langle u,v \rangle \over \langle v, v\rangle}|^2\langle v,v\rangle=\langle z ,z\rangle+{|\langle u, v \rangle |\over \langle v, v \rangle} \ge {|\langle u, v \rangle |^2\over \langle v, v \rangle}
$$
따라서
$$
\langle u,u\rangle \ge {|\langle u, v \rangle |^2\over \langle v, v \rangle}
$$
정리하면
$$
|\langle u, v \rangle |^2 \le \langle u,u\rangle \langle v, v\rangle
$$